aneris/examples/snapshot_isolation/proof/resources/wrappers.v
@@ -56,8 +56,8 @@ Section Wrapper_defs.
   Definition OwnMemKey_def k h : iProp Σ :=
     ∃ hw, ownMemUser γGauth γGsnap k hw ∗ ⌜h = to_hist hw⌝.
 
-  Definition ConnectionState_def c s : iProp Σ :=
-    ∃ sp, connection_state γGsnap γT γKnownClients c sp ∗ ⌜s = to_local_state sp⌝.
+  Definition ConnectionState_def c sa s : iProp Σ :=
+    ∃ sp, connection_state γGsnap γT γKnownClients c sa sp ∗ ⌜s = to_local_state sp⌝.
 
   Definition Seen_def k h : iProp Σ :=
     ∃ hw, ownMemSeen γGsnap k hw ∗ ⌜h = to_hist hw⌝.
