aneris/examples/snapshot_isolation/examples/causality_example/causality_example_proof.v
@@ -48,7 +48,7 @@ Section proof_of_code.
   Lemma transaction1_spec :
     ∀ (cst : val) sa,
     client_inv -∗
-    {{{ ConnectionState cst CanStart ∗ IsConnected cst }}}
+    {{{ ConnectionState cst sa CanStart ∗ IsConnected cst sa }}}
       transaction1 cst @[ip_of_address sa]
     {{{ RET #(); True }}}.
   Proof.
@@ -109,7 +109,7 @@ Section proof_of_code.
   Lemma transaction2_spec :
     ∀ (cst : val) sa,
     client_inv -∗
-    {{{ ConnectionState cst CanStart ∗ IsConnected cst }}}
+    {{{ ConnectionState cst sa CanStart ∗ IsConnected cst sa }}}
       transaction2 cst @[ip_of_address sa]
     {{{ RET #(); True }}}.
   Proof.
@@ -205,7 +205,7 @@ Section proof_of_code.
   Lemma transaction3_spec :
     ∀ (cst : val) sa,
     client_inv -∗
-    {{{ ConnectionState cst CanStart ∗ IsConnected cst }}}
+    {{{ ConnectionState cst sa CanStart ∗ IsConnected cst sa }}}
       transaction3 cst @[ip_of_address sa]
     {{{ RET #(); True }}}.
   Proof.
