aneris/examples/snapshot_isolation/instantiation/instantiation_of_init.v
@@ -1,0 +1,12 @@
+From aneris.examples.snapshot_isolation
+     Require Import snapshot_isolation_code
+                    snapshot_isolation_code_api.
+From aneris.aneris_lang Require Import resources.
+From aneris.examples.snapshot_isolation.specs Require Import user_params specs.
+From aneris.examples.snapshot_isolation.instantiation
+     Require Import snapshot_isolation_api_implementation.
+
+Global Instance SI_init_instanciation `{!anerisG Mdl Σ, !User_params} :
+    SI_init.
+Proof.
+Admitted.
